Props/FeeHolder: prove properties of withdrawBurned/Token

FeeHolder.v
@@ -20,7 +20,7 @@ Module FeeHolder.
   Section Aux.
 
     Definition wst_before_transfer
-               (wst: WorldState) (from sender token: address) (value: uint)
+               (wst: WorldState) (from to token: address) (value: uint)
     : WorldState :=
       let st := wst_feeholder_state wst in
       wst_update_feeholder
@@ -31,46 +31,51 @@ Module FeeHolder.
                                                 token from value;
         |}.
 
-    Definition transfer_withdraw
-               (wst: WorldState) (sender token: address) (value: uint)
+    Definition transfer_withdraw_succeed
+               (wst: WorldState) (to token: address) (value: uint)
       : WorldState -> list Event -> Prop :=
       fun wst' events =>
-        forall retval,
-          ERC20s.model wst
-                       (msg_transfer (wst_feeholder_addr wst) token sender value)
-                       wst' retval events.
+        ERC20s.model wst
+                     (msg_transfer (wst_feeholder_addr wst) token to value)
+                     wst' (RetBool true) events.
 
-    Definition is_authorized (wst: WorldState) (sender: address) : Prop :=
-      exists wst' events retval,
-        TradeDelegate.model wst
-                            (msg_isAddressAuthorized (wst_feeholder_addr wst) sender)
-                            wst' retval events /\
-        retval = RetBool true.
-
-    Definition withdraw_require
-               (wst: WorldState) (from sender token: address) (value: uint) :=
-      is_authorized wst sender /\
-      AA2V.get (feeholder_feeBalances (wst_feeholder_state wst))
-               (token, from) >= value /\
+    Definition is_authorized (wst: WorldState) (addr: address) : Prop :=
       exists wst' events,
-        transfer_withdraw (wst_before_transfer wst from sender token value)
-                          sender token value
-                          wst' events.
+        TradeDelegate.model wst
+                            (msg_isAddressAuthorized (wst_feeholder_addr wst) addr)
+                            wst' (RetBool true) events.
+
+    Definition has_sufficient_feebalance
+               (wst: WorldState) (from to token: address) (value: uint) :=
+      AA2V.get (feeholder_feeBalances (wst_feeholder_state wst))
+               (token, from) >= value.
+
+    Definition withdraw_require_common
+               (wst: WorldState) (from to token: address) (value: uint) :=
+      has_sufficient_feebalance wst from to token value /\
+      exists wst' events,
+        transfer_withdraw_succeed (wst_before_transfer wst from to token value)
+                                  to token value
+                                  wst' events.
+
     Definition withdraw_trans
-               (wst wst': WorldState) (retval: RetVal) (from sender token: address) (value: uint) :=
-      retval = RetNone /\
-      forall wst'' events,
-        transfer_withdraw (wst_before_transfer wst from sender token value)
-                          sender token value
-                          wst'' events ->
-        wst' = wst''.
+               (wst wst': WorldState)
+               (retval: RetVal)
+               (from to token: address)
+               (value: uint) : Prop :=
+      forall wst'' events',
+        transfer_withdraw_succeed (wst_before_transfer wst from to token value)
+                                  to token value wst'' events' ->
+        wst' = wst'' /\ retval = RetBool true.
 
     Definition withdraw_events
-               (wst: WorldState) (events: list Event) (from sender token: address) (value: uint) :=
-      forall wst' events',
-        transfer_withdraw (wst_before_transfer wst from sender token value)
-                          sender token value
-                          wst' events' ->
+               (wst: WorldState)
+               (events: list Event)
+               (from to token: address)
+               (value: uint) : Prop :=
+      forall wst'' events',
+        transfer_withdraw_succeed (wst_before_transfer wst from to token value)
+                                  to token value wst'' events' ->
         events = events' ++ (EvtTokenWithdrawn from token value :: nil).
 
   End Aux.
@@ -83,7 +88,8 @@ Module FeeHolder.
       {|
         fspec_require :=
           fun wst =>
-            withdraw_require wst (wst_feeholder_addr wst) sender token value
+            withdraw_require_common wst (wst_feeholder_addr wst) sender token value /\
+            is_authorized wst sender
         ;
 
         fspec_trans :=
@@ -105,7 +111,7 @@ Module FeeHolder.
       {|
         fspec_require :=
           fun wst =>
-            withdraw_require wst sender sender token value
+            withdraw_require_common wst sender sender token value
         ;
 
         fspec_trans :=
