Props/FeeHolderProps.v
@@ -1,0 +1,64 @@
+Require Import
+        List
+        ZArith.
+Require Import
+        Events
+        LibModel
+        Maps
+        Messages
+        States
+        Types.
+Require Import
+        ERC20
+        FeeHolder
+        TradeDelegate.
+Require Import
+        TopModel.
+
+
+Section WithdrawBurnedReqAuth.
+
+  Theorem withdrawBurn_req_auth:
+    forall sender wst,
+      ~ FeeHolder.is_authorized wst sender ->
+      forall token amount,
+        ~ (exists wst' retval events,
+              lr_step wst (MsgFeeHolder (msg_withdrawBurned sender token amount))
+                      wst' retval events).
+  Proof.
+    intros sender wst Hnot_auth token amount Hstep.
+
+    destruct Hstep as [ wst' [retval [events Hstep]]].
+    destruct Hstep as [Hreq _]; simpl in Hreq.
+    destruct Hreq as [_ Hauth].
+    congruence.
+  Qed.
+
+End WithdrawBurnedReqAuth.
+
+
+Section WithdrawTokenReqNoAuth.
+
+  Theorem withdrawToken_req_noauth:
+    forall sender wst,
+      ~ FeeHolder.is_authorized wst sender ->
+      forall token amount wst' retval events,
+        lr_step wst (MsgFeeHolder (msg_withdrawToken sender token amount))
+                wst' retval events ->
+        In (EvtTokenWithdrawn sender token amount) events.
+  Proof.
+    intros sender wst Hsender_noauth.
+    intros until events; intros Hstep.
+
+    destruct Hstep as [Hreq [_ Hevents]];
+      simpl in Hreq, Hevents.
+    destruct Hreq as [Hamount [wst'' [events' Htransfer]]].
+
+    specialize (Hevents wst'' events' Htransfer).
+    rewrite Hevents.
+
+    apply in_or_app; right.
+    constructor; auto.
+  Qed.
+
+End WithdrawTokenReqNoAuth.
